ironfleet/src/Dafny/Distributed/Protocol/Lock/RefinementProof/System.i.dfy
@@ -1,0 +1,113 @@
+include "../Node.i.dfy"
+include "Trace.i.dfy"
+include "../../../Impl/Common/SeqIsUnique.i.dfy"
+include "../../../Common/Collections/Seqs.i.dfy"
+
+module LockSystemModule {
+
+    import opened Protocol_Node_i
+    import opened LockTraceModule
+    import opened Common__SeqIsUnique_i
+    import opened Collections__Seqs_i
+
+    /////////////////////////////////////////
+    // LS_State
+    /////////////////////////////////////////
+    
+    datatype LockSystemState = LockSystemState(
+        sent_packets:set<LockPacket>,
+        states:map<LockActor, Node>
+        )
+
+    predicate LockSystemInit(config:LockConfig, s:LockSystemState)
+    {
+           s.sent_packets == {}
+        && |config| > 0
+        && SeqIsUnique(config)
+        && (forall e :: e in config <==> LockActorHost(e) in s.states)
+        && (forall index :: 0 <= index < |config| ==> NodeInit(s.states[LockActorHost(config[index])], index, config))
+    }
+
+    predicate LockSystemNextHostNext(s:LockSystemState, s':LockSystemState, actor:LockActor, ios:seq<LockIo>)
+    {
+           s' == s.(sent_packets := s'.sent_packets, states := s'.states)
+        && actor in s.states
+        && actor in s'.states
+        && s'.states == s.states[actor := s'.states[actor]]
+        && NodeNext(s.states[actor], s'.states[actor], ios)
+        && (forall p :: p in s.sent_packets ==> p in s'.sent_packets)
+        && (forall p :: p in s'.sent_packets ==> p in s.sent_packets || LockIoSend(p) in ios)
+		&& actor.LockActorHost?
+        && (forall io :: io in ios && io.LockIoReceive? ==> io.r in s.sent_packets && io.r.dst == actor.ep)
+        && (forall io :: io in ios && io.LockIoSend? ==> io.s in s'.sent_packets && io.s.src == actor.ep)
+    }
+
+    predicate LockSystemNextDeliverPacket(s:LockSystemState, s':LockSystemState, actor:LockActor, p:LockPacket)
+    {
+           p in s.sent_packets
+        && s' == s
+        && actor.LockActorNone?
+    }
+
+    predicate LockSystemNextAction(s:LockSystemState, s':LockSystemState, actor:LockActor, action:LockAction)
+    {
+        match action
+            case LockActionHostNext(ios) => LockSystemNextHostNext(s, s', actor, ios)
+            case LockActionDeliverPacket(p) => LockSystemNextDeliverPacket(s, s', actor, p)
+    }
+
+    predicate LockSystemNextEntry(s:LockSystemState, s':LockSystemState, entry:LockEntry)
+    {
+        LockSystemNextAction(s, s', entry.actor, entry.action)
+    }
+
+    predicate LockSystemNext(s:LockSystemState, s':LockSystemState)
+    {
+        exists entry :: LockSystemNextEntry(s, s', entry)
+    }
+
+    /////////////////////////////////////////////
+    // GLockSystemState: an LockSystemState augmented with
+    // a history field. This history field is
+    // initialized and updated according to
+    // GLS_Init and GLS_Next
+    /////////////////////////////////////////////
+
+    datatype GLockSystemState = GLockSystemState(
+        ls:LockSystemState,
+        history:seq<EndPoint>
+    )
+
+    predicate GLockSystemInit(config:LockConfig, s:GLockSystemState)
+    {
+           LockSystemInit(config, s.ls)
+        && s.history == [config[0]]
+    }
+
+    /////////////////////////////////////////////////////////
+    // GLockSystemNextAction is defined according to
+    // LockSystemNextAction. When a node sends a
+    // grant message, the destination of that message
+    // (as computed in NodeGrant), is appended to the history
+    /////////////////////////////////////////////////////////
+
+    predicate GLockSystemNextAction(s:GLockSystemState, s':GLockSystemState, actor:LockActor, action:LockAction)
+    {
+           LockSystemNext(s.ls, s'.ls)
+        && (if    action.LockActionHostNext?
+               && actor in s.ls.states
+               && NodeGrant(s.ls.states[actor], s'.ls.states[actor], action.ios)
+               && s.ls.states[actor].held && s.ls.states[actor].epoch < 0xFFFF_FFFF_FFFF_FFFF then
+               s'.history == s.history + [s.ls.states[actor].config[(s.ls.states[actor].my_index + 1) % |s.ls.states[actor].config|]]
+            else
+               s'.history == s.history
+           )
+    }
+
+    predicate GLockSystemNextEntry(s:GLockSystemState, s':GLockSystemState, entry:LockEntry)
+    {
+        GLockSystemNextAction(s, s', entry.actor, entry.action)
+    }
+
+}   
+
