ironfleet/src/Dafny/Distributed/Protocol/Lock/RefinementProof/Trace.i.dfy
@@ -1,0 +1,17 @@
+include "../Types.i.dfy"
+
+module LockTraceModule {
+
+    import opened Types_i
+
+    datatype LockActor = LockActorNone()
+                       | LockActorHost(ep:EndPoint)
+
+    datatype LockAction = LockActionHostNext(ios:seq<LockIo>)
+                        | LockActionDeliverPacket(p:LockPacket)
+
+    datatype LockEntry = Entry(actor:LockActor, action:LockAction)
+
+    type LockTrace = seq<LockEntry>
+
+}
